Separated "Pdec <= Pinst" proofs for singlecore and multicore

examples/ProcDecSC.v
@@ -2,13 +2,37 @@ Require Import Bool String List.
 Require Import Lib.CommonTactics Lib.ilist Lib.Word.
 Require Import Lib.Struct Lib.StringBound Lib.FMap Lib.StringEq.
 Require Import Lts.Syntax Lts.Semantics Lts.Equiv Lts.Refinement Lts.Renaming Lts.Wf.
-Require Import Lts.Renaming Lts.Specialize Lts.Inline Lts.InlineFacts_2.
+Require Import Lts.Renaming Lts.Inline Lts.InlineFacts_2.
 Require Import Lts.DecompositionZero.
 Require Import Ex.SC Ex.Fifo Ex.MemAtomic.
 Require Import Ex.ProcDec Ex.ProcDecInl Ex.ProcDecInv.
 Require Import Eqdep.
 
 Set Implicit Arguments.
+
+(** TODO: move to proper sites *)
+
+Tactic Notation "brewrite" ident(H) :=
+  match type of H with
+  | context [{| bindex:= ?s; indexb:= ?ib1 |}] =>
+    match goal with
+    | [ |- context [{| bindex:= ?s; indexb:= ?ib2 |}] ] =>
+      progress change {| bindex:= s; indexb:= ib2 |}
+      with {| bindex:= s; indexb:= ib1 |}
+    end
+  end; rewrite H.
+
+Tactic Notation "brewrite" ident(H1) "in" ident(H2) :=
+  match type of H1 with
+  | context [{| bindex:= ?s; indexb:= ?ib1 |}] =>
+    match type of H2 with
+    | context [{| bindex:= ?s; indexb:= ?ib2 |}] =>
+      progress change {| bindex:= s; indexb:= ib2 |}
+      with {| bindex:= s; indexb:= ib1 |} in H2
+    end
+  end; rewrite H1 in H2.
+
+(** TODO end *)
 
 Section ProcDecSC.
   Variables addrSize fifoSize valSize rfIdx: nat.
@@ -21,255 +45,212 @@ Section ProcDecSC.
 
   Variable n: nat.
 
-  Definition pdecN := procDecM fifoSize dec exec n.
-  Definition scN := sc dec exec opLd opSt opHt n.
+  Definition pdec := ProcDecInl.pdec fifoSize dec exec.
+  Definition pinst := pinst dec exec opLd opSt opHt.
+  Hint Unfold pdec: ModuleDefs. (* for kinline_compute *)
+  Hint Extern 1 (ModEquiv type typeUT pdec) => unfold pdec. (* for equiv_tac *)
+  Hint Extern 1 (ModEquiv type typeUT pinst) => unfold pinst. (* for equiv_tac *)
 
-  Section SingleCore.
-    Definition pdec := ProcDecInl.pdec fifoSize dec exec.
-    Definition pinst := pinst dec exec opLd opSt opHt.
-    Hint Unfold pdec: ModuleDefs. (* for kinline_compute *)
-    Hint Extern 1 (ModEquiv type typeUT pdec) => unfold pdec. (* for equiv_tac *)
-    Hint Extern 1 (ModEquiv type typeUT pinst) => unfold pinst. (* for equiv_tac *)
+  Definition pdec_pinst_ruleMap (_: RegsT) (s: string): option string :=
+    if string_dec s "reqLd" then None
+    else if string_dec s "reqSt" then None
+    else if string_dec s "repLd" then None
+    else if string_dec s "repSt" then None
+    else if string_dec s "execHt" then Some "execHt"%string
+    else if string_dec s "execNm" then Some "execNm"%string
+    else if string_dec s "processLd" then Some "execLd"%string
+    else if string_dec s "processSt" then Some "execSt"%string
+    else None.
 
-    Definition pdec_pinst_ruleMap (_: RegsT) (s: string): option string :=
-      if string_dec s "reqLd" then None
-      else if string_dec s "reqSt" then None
-      else if string_dec s "repLd" then None
-      else if string_dec s "repSt" then None
-      else if string_dec s "execHt" then Some "execHt"%string
-      else if string_dec s "execNm" then Some "execNm"%string
-      else if string_dec s "processLd" then Some "execLd"%string
-      else if string_dec s "processSt" then Some "execSt"%string
-      else None.
-    
-    Definition pdec_pinst_regMap (r: RegsT): RegsT.
-    Proof.
-      kgetv "pc"%string pcv r (Bit addrSize) (M.empty (sigT (fullType type))).
-      kgetv "rf"%string rfv r (Vector (Bit valSize) rfIdx) (M.empty (sigT (fullType type))).
-      kgetv "Outs.empty"%string oev r Bool (M.empty (sigT (fullType type))).
-      kgetv "Outs.elt"%string oelv r (Vector (memAtomK addrSize valSize) fifoSize)
-            (M.empty (sigT (fullType type))).
-      kgetv "Outs.deqP"%string odv r (Bit fifoSize) (M.empty (sigT (fullType type))).
-      refine (if oev then _ else _).
-
-      - (* Outs.empty = true *)
-        refine (M.add "pc"%string _
-                      (M.add "rf"%string _
-                             (M.empty _))).
-        + exact (existT _ _ pcv).
-        + exact (existT _ _ rfv).
-
-      - (* Outs.empty = false *)
-        refine (M.add "pc"%string _
-                      (M.add "rf"%string _
-                             (M.empty _))).
-        + exact (existT _ _ (getNextPc exec _ pcv rfv (dec _ rfv pcv))).
-        + pose proof (dec _ rfv pcv ``"opcode") as opc.
-          destruct (weq opc (evalConstT opLd)).
-          * refine (existT _ (SyntaxKind (Vector (Bit valSize) rfIdx)) _); simpl.
-            exact (fun a => if weq a (dec _ rfv pcv ``"reg")
-                            then (oelv odv) ``"value"
-                            else rfv a).
-          * refine (existT _ _ rfv).
-    Defined.
-
-    Ltac regMap_red :=
-      unfold pdec_pinst_regMap;
-      repeat
-        (try match goal with
-             | [H: M.find ?k ?m = _ |- context[M.find ?k ?m] ] => rewrite H
-             | [ |- context[decKind ?k ?k] ] =>
-               rewrite kind_eq; unfold eq_rect_r, eq_rect, eq_sym
-             end;
-         dest; try subst;
-         try findReify).
-
-    Tactic Notation "brewrite" ident(H1) "in" ident(H2) :=
-      match type of H1 with
-      | context [{| bindex:= ?s; indexb:= ?ib1 |}] =>
-        match type of H2 with
-        | context [{| bindex:= ?s; indexb:= ?ib2 |}] =>
-          progress change {| bindex:= s; indexb:= ib2 |}
-          with {| bindex:= s; indexb:= ib1 |} in H2
-        end
-      end; rewrite H1 in H2.
-
-    Lemma pdec_refines_pinst: pdec <<== pinst.
-    Proof.
-      admit.
-      (* apply traceRefines_inlining_left; auto. *)
-      (* unfold pdec; rewrite <-pdecInl_equal. *)
-      (* split; [|reflexivity]. *)
-
-      (* kdecompose_nodefs pdec_pinst_regMap pdec_pinst_ruleMap. *)
-
-      (* - unfold initRegs, getRegInits; simpl; clear. *)
-      (*   regMap_red. *)
-      (*   reflexivity. *)
-      (* - auto. *)
-      (* - auto. *)
-      (* - intros. *)
-      (*   pose proof (procDec_inv_0_ok H). *)
-      (*   pose proof (procDec_inv_1_ok H). *)
-      (*   clear H. *)
-      (*   inv H0; CommonTactics.dest_in. *)
-
-      (*   + inv H; invertActionRep. *)
-      (*     eexists; split. *)
-      (*     * econstructor. *)
-      (*     * inv_red; simpl_find. *)
-      (*       dest_or3; inv_contra. *)
-      (*       regMap_red. *)
-      (*       mred. *)
-
-      (*   + inv H0; invertActionRep. *)
-      (*     eexists; split. *)
-      (*     * econstructor. *)
-      (*     * inv_red; simpl_find. *)
-      (*       dest_or3; inv_contra. *)
-      (*       regMap_red. *)
-      (*       mred. *)
-
-      (*   + inv H; invertActionRep. *)
-      (*     eexists; split. *)
-      (*     * econstructor. *)
-      (*     * inv_red; simpl_find. *)
-      (*       dest_or3; inv_contra. *)
-      (*       regMap_red. *)
-
-      (*       destruct (weq (x2 ^+ $ (1)) (x2 ^+ $ (1))); [|elim n0; reflexivity]. *)
-      (*       clear -H9; meq. *)
-          
-      (*   + inv H0; invertActionRep. *)
-      (*     eexists; split. *)
-      (*     * econstructor. *)
-      (*     * inv_red; simpl_find. *)
-      (*       dest_or3; inv_contra. *)
-      (*       regMap_red. *)
-
-      (*       destruct (weq (x2 ^+ $ (1)) (x2 ^+ $ (1))); [|elim n0; reflexivity]. *)
-      (*       clear -H9; meq. *)
-
-      (*       brewrite e in e0. *)
-      (*       inv e0. *)
-          
-      (*   + inv H; invertActionRep. *)
-      (*     eexists; split. *)
-      (*     * inv_red; simpl_find. *)
-      (*       dest_or3; inv_contra. *)
-      (*       regMap_red. *)
-
-      (*       eapply SingleRule; [simpl; tauto|]. *)
-      (*       repeat econstructor. *)
-      (*       auto. *)
-      (*     * meq. *)
-
-      (*   + inv H0; invertActionRep. *)
-      (*     inv_red; simpl_find. *)
-      (*     dest_or3; inv_contra. *)
-      (*     regMap_red. *)
-          
-      (*     eexists; split. *)
-      (*     * eapply SingleRule; [simpl; tauto|]. *)
-      (*       repeat econstructor. *)
-      (*       simpl; apply negb_true_iff; auto. *)
-      (*     * meq. *)
-
-      (*   + inv H; invertActionRep. *)
-      (*     inv_red; simpl_find. *)
-      (*     dest_or3; inv_contra. *)
-      (*     unfold memAtomK, atomK in *. *)
-      (*     regMap_red. *)
-              
-      (*     eexists; split. *)
-      (*     * eapply SingleRule; [simpl; tauto|]. *)
-      (*       repeat econstructor. *)
-      (*       { simpl in *; clear -H0 H7. *)
-      (*         repeat find_if_inside; intuition idtac. *)
-      (*         elim n; clear n; rewrite <-e; auto. *)
-      (*       } *)
-      (*       { rewrite idElementwiseId; unfold id. *)
-      (*         do 3 f_equal. *)
-      (*         simpl; boundedMapTac. *)
-      (*         { clear -H7. *)
-      (*           find_if_inside; auto; inv H7. *)
-      (*         } *)
-      (*         { clear -H3 H7. *)
-      (*           repeat find_if_inside; intuition idtac; inv H7. *)
-      (*         } *)
-      (*       } *)
-      (*     * clear -H0 H7; meq. *)
-      (*       elim n; clear n. *)
-      (*       simpl; rewrite <-e; auto. *)
-
-      (*   + inv H0; invertActionRep. *)
-      (*     inv_red; simpl_find. *)
-      (*     dest_or3; inv_contra. *)
-      (*     unfold memAtomK, atomK in *. *)
-      (*     regMap_red. *)
-
-      (*     eexists; split. *)
-      (*     * eapply SingleRule; [simpl; tauto|]. *)
-      (*       repeat econstructor. *)
-      (*       { simpl in *; clear -H0 H7. *)
-      (*         repeat find_if_inside; intuition idtac. *)
-      (*         elim n; clear n; rewrite <-e; auto. *)
-      (*       } *)
-      (*       { rewrite idElementwiseId; unfold id. *)
-      (*         do 3 f_equal. *)
-      (*         simpl; boundedMapTac. *)
-      (*         { clear -H7. *)
-      (*           find_if_inside; intuition idtac. *)
-      (*           inv H7. *)
-      (*         } *)
-      (*         { clear -H3 H7. *)
-      (*           repeat find_if_inside; intuition idtac. *)
-      (*           { brewrite e0 in e; inv e. } *)
-      (*           { inv H7. } *)
-      (*           { inv H7. } *)
-      (*         } *)
-      (*       } *)
-      (*     * clear -H0 H7; meq. *)
-      (*       rewrite e0 in H0. *)
-      (*       brewrite e in H0. *)
-      (*       inv H0. *)
-    Qed.
-
-  End SingleCore.
-
-  Lemma pdecN_refines_scN: traceRefines (liftToMap1 (@idElementwise _)) pdecN scN.
+  Definition pdec_pinst_regMap (r: RegsT): RegsT.
   Proof.
-    apply traceRefines_modular_interacting with (vp:= (@idElementwise _)); auto.
-    - admit.
-    - admit.
-    - admit. 
-    - admit.
-    - admit.
-    - admit.
-    - admit.
-    - admit.
-    - apply duplicate_defCallSub.
-      vm_compute; split; intros; intuition idtac.
-    - apply DefCallSub_refl.
-    - repeat split.
-    - (* TODO: a general lemma for duplication-refinement: implement in Specialize.v *)
-      induction n; simpl; intros.
-      + apply specialized_2.
-        * intros; vm_compute.
-          (* intro; dest. *)
-          (* repeat *)
-          (*   match goal with *)
-          (*   | [H: _ \/ _ |- _] => destruct H *)
-          (*   end; subst; try discriminate; auto. *)
-          (* TODO: takes a time ... *)
-          admit.
-        * intros; vm_compute; admit.
-        * apply traceRefines_label_map with (p:= liftToMap1 (@idElementwise _)); auto.
-          { admit. }
-          { admit. (* apply pdec_refines_pinst. *) }
-      + admit. (* apply traceRefines_modular_noninteracting. *)
-    - rewrite idElementwiseId; apply traceRefines_refl.
+    kgetv "pc"%string pcv r (Bit addrSize) (M.empty (sigT (fullType type))).
+    kgetv "rf"%string rfv r (Vector (Bit valSize) rfIdx) (M.empty (sigT (fullType type))).
+    kgetv "Outs.empty"%string oev r Bool (M.empty (sigT (fullType type))).
+    kgetv "Outs.elt"%string oelv r (Vector (memAtomK addrSize valSize) fifoSize)
+          (M.empty (sigT (fullType type))).
+    kgetv "Outs.deqP"%string odv r (Bit fifoSize) (M.empty (sigT (fullType type))).
+    refine (if oev then _ else _).
 
+    - (* Outs.empty = true *)
+      refine (M.add "pc"%string _
+                    (M.add "rf"%string _
+                           (M.empty _))).
+      + exact (existT _ _ pcv).
+      + exact (existT _ _ rfv).
+
+    - (* Outs.empty = false *)
+      refine (M.add "pc"%string _
+                    (M.add "rf"%string _
+                           (M.empty _))).
+      + exact (existT _ _ (getNextPc exec _ pcv rfv (dec _ rfv pcv))).
+      + pose proof (dec _ rfv pcv ``"opcode") as opc.
+        destruct (weq opc (evalConstT opLd)).
+        * refine (existT _ (SyntaxKind (Vector (Bit valSize) rfIdx)) _); simpl.
+          exact (fun a => if weq a (dec _ rfv pcv ``"reg")
+                          then (oelv odv) ``"value"
+                          else rfv a).
+        * refine (existT _ _ rfv).
+  Defined.
+
+  Ltac regMap_red :=
+    unfold pdec_pinst_regMap;
+    repeat
+      (try match goal with
+           | [H: M.find ?k ?m = _ |- context[M.find ?k ?m] ] => rewrite H
+           | [ |- context[decKind ?k ?k] ] =>
+             rewrite kind_eq; unfold eq_rect_r, eq_rect, eq_sym
+           end;
+       dest; try subst;
+       try findReify).
+
+  Lemma pdec_refines_pinst: pdec <<== pinst.
+  Proof.
+    admit.
+    (* apply traceRefines_inlining_left; auto. *)
+    (* unfold pdec; rewrite <-pdecInl_equal. *)
+    (* split; [|reflexivity]. *)
+
+    (* kdecompose_nodefs pdec_pinst_regMap pdec_pinst_ruleMap. *)
+
+    (* - unfold initRegs, getRegInits; simpl; clear. *)
+    (*   regMap_red. *)
+    (*   reflexivity. *)
+    (* - auto. *)
+    (* - auto. *)
+    (* - intros. *)
+    (*   pose proof (procDec_inv_0_ok H). *)
+    (*   pose proof (procDec_inv_1_ok H). *)
+    (*   clear H. *)
+    (*   inv H0; CommonTactics.dest_in. *)
+
+    (*   + inv H; invertActionRep. *)
+    (*     eexists; split. *)
+    (*     * econstructor. *)
+    (*     * inv_red; simpl_find. *)
+    (*       dest_or3; inv_contra. *)
+    (*       regMap_red. *)
+    (*       mred. *)
+
+    (*   + inv H0; invertActionRep. *)
+    (*     eexists; split. *)
+    (*     * econstructor. *)
+    (*     * inv_red; simpl_find. *)
+    (*       dest_or3; inv_contra. *)
+    (*       regMap_red. *)
+    (*       mred. *)
+
+    (*   + inv H; invertActionRep. *)
+    (*     eexists; split. *)
+    (*     * econstructor. *)
+    (*     * inv_red; simpl_find. *)
+    (*       dest_or3; inv_contra. *)
+    (*       regMap_red. *)
+
+    (*       destruct (weq (x2 ^+ $ (1)) (x2 ^+ $ (1))); [|elim n0; reflexivity]. *)
+    (*       clear -H9. *)
+    (*       match goal with *)
+    (*       | [H: (if ?c then true else false) = true |- _] => destruct c; [|inv H] *)
+    (*       end. *)
+    (*       brewrite e. *)
+    (*       reflexivity. *)
+          
+    (*   + inv H0; invertActionRep. *)
+    (*     eexists; split. *)
+    (*     * econstructor. *)
+    (*     * inv_red; simpl_find. *)
+    (*       dest_or3; inv_contra. *)
+    (*       regMap_red. *)
+
+    (*       destruct (weq (x2 ^+ $ (1)) (x2 ^+ $ (1))); [|elim n0; reflexivity]. *)
+    (*       clear -H9. *)
+    (*       match goal with *)
+    (*       | [H: (if ?c then true else false) = true |- _] => destruct c; [|inv H] *)
+    (*       end. *)
+    (*       brewrite e. *)
+    (*       reflexivity. *)
+          
+    (*   + inv H; invertActionRep. *)
+    (*     eexists; split. *)
+    (*     * inv_red; simpl_find. *)
+    (*       dest_or3; inv_contra. *)
+    (*       regMap_red. *)
+
+    (*       eapply SingleRule; [simpl; tauto|]. *)
+    (*       repeat econstructor. *)
+    (*       auto. *)
+    (*     * do 2 rewrite M.union_empty_L. *)
+    (*       reflexivity. *)
+
+    (*   + inv H0; invertActionRep. *)
+    (*     inv_red; simpl_find. *)
+    (*     dest_or3; inv_contra. *)
+    (*     regMap_red. *)
+        
+    (*     eexists; split. *)
+    (*     * eapply SingleRule; [simpl; tauto|]. *)
+    (*       repeat econstructor. *)
+    (*       simpl; apply negb_true_iff; auto. *)
+    (*     * meq. *)
+
+    (*   + inv H; invertActionRep. *)
+    (*     inv_red; simpl_find. *)
+    (*     dest_or3; inv_contra. *)
+    (*     unfold memAtomK, atomK in *. *)
+    (*     regMap_red. *)
+        
+    (*     eexists; split. *)
+    (*     * eapply SingleRule; [simpl; tauto|]. *)
+    (*       repeat econstructor. *)
+    (*       { simpl in *; clear -H0 H7. *)
+    (*         repeat find_if_inside; intuition idtac. *)
+    (*         elim n; clear n; rewrite <-e; auto. *)
+    (*       } *)
+    (*       { rewrite idElementwiseId; unfold id. *)
+    (*         do 3 f_equal. *)
+    (*         simpl; boundedMapTac. *)
+    (*         { clear -H7. *)
+    (*           find_if_inside; auto; inv H7. *)
+    (*         } *)
+    (*         { clear -H3 H7. *)
+    (*           repeat find_if_inside; intuition idtac; inv H7. *)
+    (*         } *)
+    (*       } *)
+    (*     * clear -H0 H7; meq. *)
+    (*       elim n; clear n. *)
+    (*       simpl; rewrite <-e; auto. *)
+
+    (*   + inv H0; invertActionRep. *)
+    (*     inv_red; simpl_find. *)
+    (*     dest_or3; inv_contra. *)
+    (*     unfold memAtomK, atomK in *. *)
+    (*     regMap_red. *)
+
+    (*     eexists; split. *)
+    (*     * eapply SingleRule; [simpl; tauto|]. *)
+    (*       repeat econstructor. *)
+    (*       { simpl in *; clear -H0 H7. *)
+    (*         repeat find_if_inside; intuition idtac. *)
+    (*         elim n; clear n; rewrite <-e; auto. *)
+    (*       } *)
+    (*       { rewrite idElementwiseId; unfold id. *)
+    (*         do 3 f_equal. *)
+    (*         simpl; boundedMapTac. *)
+    (*         { clear -H7. *)
+    (*           find_if_inside; intuition idtac. *)
+    (*           inv H7. *)
+    (*         } *)
+    (*         { clear -H3 H7. *)
+    (*           repeat find_if_inside; intuition idtac. *)
+    (*           { brewrite e0 in e; inv e. } *)
+    (*           { inv H7. } *)
+    (*           { inv H7. } *)
+    (*         } *)
+    (*       } *)
+    (*     * clear -H0 H7; meq. *)
+    (*       rewrite e0 in H0. *)
+    (*       brewrite e in H0. *)
+    (*       inv H0. *)
   Qed.
 
 End ProcDecSC.
