examples/ProcDecSCN.v
@@ -1,0 +1,60 @@
+Require Import Bool String List.
+Require Import Lib.CommonTactics Lib.ilist Lib.Word.
+Require Import Lib.Struct Lib.StringBound Lib.FMap Lib.StringEq.
+Require Import Lts.Syntax Lts.Semantics Lts.Equiv Lts.Refinement Lts.Renaming Lts.Wf.
+Require Import Lts.Renaming Lts.Specialize.
+Require Import Ex.SC Ex.Fifo Ex.MemAtomic.
+Require Import Ex.ProcDec Ex.ProcDecInl Ex.ProcDecInv Ex.ProcDecSC.
+
+Set Implicit Arguments.
+
+Section ProcDecSCN.
+  Variables addrSize fifoSize valSize rfIdx: nat.
+
+  Variable dec: DecT 2 addrSize valSize rfIdx.
+  Variable exec: ExecT 2 addrSize valSize rfIdx.
+  Hypotheses (HdecEquiv: DecEquiv dec)
+             (HexecEquiv_1: ExecEquiv_1 dec exec)
+             (HexecEquiv_2: ExecEquiv_2 dec exec).
+
+  Variable n: nat.
+
+  Definition pdecN := procDecM fifoSize dec exec n.
+  Definition scN := sc dec exec opLd opSt opHt n.
+
+  Lemma pdecN_refines_scN: traceRefines (liftToMap1 (@idElementwise _)) pdecN scN.
+  Proof.
+    apply traceRefines_modular_interacting with (vp:= (@idElementwise _)); auto.
+    - admit.
+    - admit.
+    - admit. 
+    - admit.
+    - admit.
+    - admit.
+    - admit.
+    - admit.
+    - apply duplicate_defCallSub.
+      vm_compute; split; intros; intuition idtac.
+    - apply DefCallSub_refl.
+    - repeat split.
+    - (* TODO: a general lemma for duplication-refinement: implement in Specialize.v *)
+      induction n; simpl; intros.
+      + apply specialized_2.
+        * intros; vm_compute.
+          (* intro; dest. *)
+          (* repeat *)
+          (*   match goal with *)
+          (*   | [H: _ \/ _ |- _] => destruct H *)
+          (*   end; subst; try discriminate; auto. *)
+          (* TODO: takes a time ... *)
+          admit.
+        * intros; vm_compute; admit.
+        * apply traceRefines_label_map with (p:= liftToMap1 (@idElementwise _)); auto.
+          { admit. }
+          { admit. (* apply pdec_refines_pinst. *) }
+      + admit. (* apply traceRefines_modular_noninteracting. *)
+    - rewrite idElementwiseId; apply traceRefines_refl.
+  Qed.
+
+End ProcDecSCN.
+
